compiler/src/compilerExamples/SoftmulBedrock2.v
@@ -1,0 +1,58 @@
+Require Import ZArith coqutil.Z.div_mod_to_equations.
+Require Import bedrock2.NotationsCustomEntry.
+Import Syntax BinInt String List.ListNotations ZArith.
+Require Import coqutil.Z.Lia.
+Require Import bedrock2Examples.rpmul.
+Local Open Scope string_scope. Local Open Scope Z_scope. Local Open Scope list_scope.
+
+(* Variant of "ipow" implementing multiplication in terms of addition instead
+* of exponentiation in terms of multiplication. *)
+
+Definition softmul :=
+  ("softmul", (["inst"; "a_regs"], @nil String.string, bedrock_func_body:(
+  (* TODO for Andres *)
+  a = $2;
+  b = $3;
+  unpack! c = rpmul(a, b)
+))).
+
+From bedrock2 Require Import Semantics BasicC32Semantics WeakestPrecondition ProgramLogic.
+From coqutil Require Import Word.Properties Word.Interface Tactics.letexists.
+Require Import riscv.Spec.Decode riscv.Utility.Utility.
+Require Import bedrock2.SepAutoArray bedrock2.SepAuto.
+Open Scope bool_scope.
+
+(* like (decode RV32I), but additionally also accepts the Mul instruction
+   (but no other instructions from the M extension) *)
+Definition mdecode(inst: Z): Instruction :=
+  let opcode := bitSlice inst 0 7 in
+  let rd := bitSlice inst 7 12 in
+  let funct3 := bitSlice inst 12 15 in
+  let rs1 := bitSlice inst 15 20 in
+  let rs2 := bitSlice inst 20 25 in
+  let funct7 := bitSlice inst 25 32 in
+  if (opcode =? opcode_OP) && (funct3 =? funct3_MUL) && (funct7 =? funct7_MUL)
+  then MInstruction (Mul rd rs1 rs2)
+  else decode RV32I inst.
+
+Definition idecode: Z -> Instruction := decode RV32I.
+
+#[export] Instance spec_of_softmul : spec_of "softmul" :=
+  fnspec! "softmul" inst a_regs / rd rs1 rs2 regvals R,
+  { requires t m :=
+      mdecode (word.unsigned inst) = MInstruction (Mul rd rs1 rs2) /\
+      List.length regvals = 32%nat /\
+      seps [a_regs |-> word_array regvals; R] m;
+      (* Alternative way of expressing the length constraint:
+      seps [a_regs |-> with_len 32 word_array regvals; R] m; *)
+    ensures t' m' :=
+      t = t' /\
+      seps [a_regs |-> word_array (List.upd regvals (Z.to_nat rd) (word.mul
+               (List.nth (Z.to_nat rs1) regvals default)
+               (List.nth (Z.to_nat rs2) regvals default))); R] m
+ }.
+
+Lemma softmul_ok : program_logic_goal_for_function! softmul.
+Proof.
+  (* TODO for Andres *)
+Admitted.
